\documentclass[10pt,fleqn]{article}
\newcommand{\name}[1]{\def\psettitlename{#1}}
\newcommand{\course}[1]{\def\psettitlecourse{#1}}
\newcommand{\rsection}[1]{\def\psettitlersection{#1}}
\newcommand{\psetnum}[1]{\def\psettitlepsetnum{#1}}
%\usepackage[journal=rsc]{chemstyle}
%\usepackage{mhchem}
\usepackage{amsmath}
\usepackage{amssymb}
\usepackage{amsfonts}
\usepackage{esint}
\usepackage{bbm}
\usepackage{amscd}
\usepackage{picinpar}
\usepackage[pdftex]{graphicx}
\usepackage{tikz}
\usepackage{indentfirst}
\usepackage{wrapfig}
\usepackage{units}
\usepackage{textcomp}
\usepackage[utf8x]{inputenc}
% \usepackage{feyn}
\usepackage{feynmp}
\usetikzlibrary{
  arrows,
  calc,
  decorations.pathmorphing,
  decorations.pathreplacing,
  decorations.markings,
  fadings,
  positioning,
  shapes
}

\DeclareGraphicsRule{*}{mps}{*}{}
\newcommand{\ud}{\mathrm{d}}
\newcommand{\ue}{\mathrm{e}}
\newcommand{\ui}{\mathrm{i}}
\newcommand{\res}{\mathrm{Res}}
\newcommand{\Tr}{\mathrm{Tr}}
\newcommand{\dsum}{\displaystyle\sum}
\newcommand{\dprod}{\displaystyle\prod}
\newcommand{\dlim}{\displaystyle\lim}
\newcommand{\dint}{\displaystyle\int}
\newcommand{\fsno}[1]{{\!\not\!{#1}}}
\newcommand{\eqar}[1]
{
  \begin{align*}
    #1
  \end{align*}
}
\newcommand{\texp}[2]{\ensuremath{{#1}\times10^{#2}}}
\newcommand{\dexp}[2]{\ensuremath{{#1}\cdot10^{#2}}}
\newcommand{\eval}[2]{{\left.{#1}\right|_{#2}}}
\newcommand{\paren}[1]{{\left({#1}\right)}}
\newcommand{\lparen}[1]{{\left({#1}\right.}}
\newcommand{\rparen}[1]{{\left.{#1}\right)}}
\newcommand{\abs}[1]{{\left|{#1}\right|}}
\newcommand{\sqr}[1]{{\left[{#1}\right]}}
\newcommand{\crly}[1]{{\left\{{#1}\right\}}}
\newcommand{\angl}[1]{{\left\langle{#1}\right\rangle}}
\newcommand{\tpdiff}[4][{}]{{\paren{\frac{\partial^{#1} {#2}}{\partial {#3}{}^{#1}}}_{#4}}}
\newcommand{\tpsdiff}[4][{}]{{\paren{\frac{\partial^{#1}}{\partial {#3}{}^{#1}}{#2}}_{#4}}}
\newcommand{\pdiff}[3][{}]{{\frac{\partial^{#1} {#2}}{\partial {#3}{}^{#1}}}}
\newcommand{\diff}[3][{}]{{\frac{\ud^{#1} {#2}}{\ud {#3}{}^{#1}}}}
\newcommand{\psdiff}[3][{}]{{\frac{\partial^{#1}}{\partial {#3}{}^{#1}} {#2}}}
\newcommand{\sdiff}[3][{}]{{\frac{\ud^{#1}}{\ud {#3}{}^{#1}} {#2}}}
\newcommand{\tpddiff}[4][{}]{{\left(\dfrac{\partial^{#1} {#2}}{\partial {#3}{}^{#1}}\right)_{#4}}}
\newcommand{\tpsddiff}[4][{}]{{\paren{\dfrac{\partial^{#1}}{\partial {#3}{}^{#1}}{#2}}_{#4}}}
\newcommand{\pddiff}[3][{}]{{\dfrac{\partial^{#1} {#2}}{\partial {#3}{}^{#1}}}}
\newcommand{\ddiff}[3][{}]{{\dfrac{\ud^{#1} {#2}}{\ud {#3}{}^{#1}}}}
\newcommand{\psddiff}[3][{}]{{\frac{\partial^{#1}}{\partial{}^{#1} {#3}} {#2}}}
\newcommand{\sddiff}[3][{}]{{\frac{\ud^{#1}}{\ud {#3}{}^{#1}} {#2}}}
\usepackage{fancyhdr}
\usepackage{multirow}
\usepackage{fontenc}
%\usepackage{tipa}
\usepackage{ulem}
\usepackage{color}
\usepackage{cancel}
\newcommand{\hcancel}[2][black]{\setbox0=\hbox{#2}%
\rlap{\raisebox{.45\ht0}{\textcolor{#1}{\rule{\wd0}{1pt}}}}#2}
\pagestyle{fancy}
\setlength{\headheight}{67pt}
\fancyhead{}
\fancyfoot{}
\fancyfoot[C]{\thepage}
\fancyhead[R]
{
\psettitlename \\
\psettitlecourse{} Problem Set \psettitlepsetnum \\
\ifx\psettitlersection\empty
\else
Recitation Section \psettitlersection
\fi
}
\renewcommand{\footruleskip}{0pt}
\renewcommand{\headrulewidth}{0.4pt}
\renewcommand{\footrulewidth}{0pt}
\addtolength{\hoffset}{-1.3cm}
\addtolength{\voffset}{-2cm}
\addtolength{\textwidth}{3cm}
\addtolength{\textheight}{2.5cm}
\renewcommand{\footskip}{10pt}
\setlength{\headwidth}{\textwidth}
\setlength{\headsep}{20pt}
\setlength{\marginparwidth}{0pt}
\parindent=0pt
\psetnum{4}
\input{../head}
\begin{document}
\section{}
\subsection{}
Define
\eqar{
  Y\paren{x, y}=&\frac{x^ny^{n-1}+x^{n-1}y^n}{\sqrt{2n!\paren{n-1}!}}
  \intertext{when $\sqr{x, y}=0$}
  Y\paren{x, y}=&x^{n-1}y^{n-1}\frac{x+y}{\sqrt{2n!\paren{n-1}!}}
  \intertext{we also have, for any number $\lambda$}
  Y\paren{\lambda x, \lambda y}=&\lambda^{2n-1}Y\paren{x, y}
}
Before the first beam splitter
\eqar{
  |\psi_0\rangle=&Y\paren{a^\dagger, b^\dagger}|0, 0\rangle\\
  =&{a^\dagger}^{n-1}{b^\dagger}^{n-1}\frac{{a^\dagger}+{b^\dagger}}{\sqrt{2n!\paren{n-1}!}}|0, 0\rangle
  \intertext{After the first beam splitter}
  |\psi_1\rangle=&B|\psi_0\rangle\\
  =&BY\paren{a^\dagger, b^\dagger}B^\dagger|0, 0\rangle\\
  =&Y\paren{Ba^\dagger B^\dagger, Bb^\dagger B^\dagger}|0, 0\rangle\\
  =&\frac{\sqrt{2}}{2^n}Y\paren{a^\dagger-\ui b^\dagger, b^\dagger-\ui a^\dagger}|0, 0\rangle\\
  =&\paren{a^\dagger-\ui b^\dagger}^{n-1}\paren{b^\dagger-\ui a^\dagger}^{n-1}\frac{a^\dagger-\ui b^\dagger+b^\dagger-\ui a^\dagger}{2^{n}\sqrt{n!\paren{n-1}!}}|0, 0\rangle\\
  =&\paren{-\ui}^{n-1}\paren{1-\ui}\paren{{a^\dagger}^2+{b^\dagger}^2}^{n-1}\frac{a^\dagger+b^\dagger}{2^{n}\sqrt{n!\paren{n-1}!}}|0, 0\rangle
  \intertext{After phase shift}
  |\psi_2\rangle=&\frac{\sqrt{2}}{2^n}Y\paren{\ue^{-\ui\phi}a^\dagger-\ui b^\dagger, b^\dagger-\ui \ue^{-\ui\phi}a^\dagger}|0, 0\rangle\\
  =&\paren{-\ui}^{n-1}\paren{1-\ui}\paren{\ue^{-2\ui\phi}{a^\dagger}^2+{b^\dagger}^2}^{n-1}\frac{\ue^{-\ui\phi}a^\dagger+b^\dagger}{2^{n}\sqrt{n!\paren{n-1}!}}|0, 0\rangle
  \intertext{Output}
  |\psi_3\rangle=&B^\dagger|\psi_2\rangle\\
  =&\frac{\ue^{-\ui\phi\paren{n-1/2}}}{2^{2n-1}}Y\paren{\ue^{-\ui\phi/2}\paren{a^\dagger+\ui b^\dagger}-\ui \ue^{\ui\phi/2}\paren{b^\dagger+\ui a^\dagger}, \ue^{\ui\phi/2}\paren{b^\dagger+\ui a^\dagger}-\ui \ue^{-\ui\phi/2}\paren{a^\dagger+\ui b^\dagger}}|0, 0\rangle\\
  =&\frac{\ue^{-\ui\phi\paren{n-1/2}}}{2^{2n-1}}Y\paren{2\cos\frac{\phi}{2}a^\dagger+2\sin\frac{\phi}{2}b^\dagger, 2\cos\frac{\phi}{2}b^\dagger-2\sin\frac{\phi}{2}a^\dagger}|0, 0\rangle\\
  =&\ue^{-\ui\phi\paren{n-1/2}}Y\paren{\cos\frac{\phi}{2}a^\dagger+\sin\frac{\phi}{2}b^\dagger, \cos\frac{\phi}{2}b^\dagger-\sin\frac{\phi}{2}a^\dagger}|0, 0\rangle\\
  =&\frac{\ue^{-\ui\phi\paren{n-1/2}}}{\sqrt{2n!\paren{n-1}!}}
  \paren{\cos\frac{\phi}{2}a^\dagger+\sin\frac{\phi}{2}b^\dagger}^{n-1}
  \paren{\cos\frac{\phi}{2}b^\dagger-\sin\frac{\phi}{2}a^\dagger}^{n-1}\\
  &\paren{\cos\frac{\phi}{2}a^\dagger+\sin\frac{\phi}{2}b^\dagger+\cos\frac{\phi}{2}b^\dagger-\sin\frac{\phi}{2}a^\dagger}
  |0, 0\rangle
  \intertext{For $\phi=0$}
  |\phi_3\rangle_0=&\frac{1}{\sqrt{n!\paren{n-1}!}}
  {a^\dagger}^{n-1} {b^\dagger}^{n-1}
  \frac{a^\dagger+b^\dagger}{\sqrt2}|0, 0\rangle\\
  =&|\phi_0\rangle
}
\subsection{}
Let
\eqar{
  a'=&\cos\frac{\phi}{2}a+\sin\frac{\phi}{2}b\\
  b'=&\cos\frac{\phi}{2}b-\sin\frac{\phi}{2}a
  \intertext{then}
  a'^\dagger=&\cos\frac{\phi}{2}a^\dagger+\sin\frac{\phi}{2}b^\dagger\\
  b'^\dagger=&\cos\frac{\phi}{2}b^\dagger-\sin\frac{\phi}{2}a^\dagger\\
  a=&\cos\frac{\phi}{2}a'-\sin\frac{\phi}{2}b'\\
  b=&\cos\frac{\phi}{2}b'+\sin\frac{\phi}{2}a'\\
  a^\dagger=&\cos\frac{\phi}{2}a'^\dagger-\sin\frac{\phi}{2}b'^\dagger\\
  b^\dagger=&\cos\frac{\phi}{2}b'^\dagger+\sin\frac{\phi}{2}a'^\dagger\\
  \sqr{a', a'^\dagger}=&1\\
  \sqr{b', b'^\dagger}=&1\\
  |\phi_3\rangle=&\frac{\ue^{-\ui\phi\paren{n-1/2}}}{\sqrt{n!\paren{n-1}!}}
  {a'^\dagger}^{n-1} {b'^\dagger}^{n-1}
  \frac{a'^\dagger+b'^\dagger}{\sqrt2}|0, 0\rangle
  \intertext{}
  M=&a^\dagger a-b^\dagger b\\
  =&\paren{\cos\frac{\phi}{2}a'^\dagger-\sin\frac{\phi}{2}b'^\dagger}\paren{\cos\frac{\phi}{2}a'-\sin\frac{\phi}{2}b'}-\paren{\cos\frac{\phi}{2}b'^\dagger+\sin\frac{\phi}{2}a'^\dagger}\paren{\cos\frac{\phi}{2}b'+\sin\frac{\phi}{2}a'}\\
  =&\cos^2\frac{\phi}{2}a'^\dagger a'+\sin^2\frac{\phi}{2}b'^\dagger b'
  -\sin\frac{\phi}{2}\cos\frac{\phi}{2}\paren{a'b'^\dagger+a'^\dagger b'}\\
  &-\cos^2\frac{\phi}{2}b'^\dagger b'
  -\sin\frac{\phi}{2}\cos\frac{\phi}{2}a'^\dagger b'
  -\sin\frac{\phi}{2}\cos\frac{\phi}{2}a' b'^\dagger
  -\sin^2\frac{\phi}{2}a'^\dagger a'\\
  =&\cos\phi\paren{a'^\dagger a'-b'^\dagger b'}-\sin\phi\paren{a'b'^\dagger+a'^\dagger b'}
  \intertext{Mean}
  \angl{M}=&\frac{1}{2n!\paren{n-1}!}
  \langle0, 0|
  {a'}^{n-1} {b'}^{n-1}
  \paren{a'+b'}
  \paren{\cos\phi\paren{a'^\dagger a'-b'^\dagger b'}-\sin\phi\paren{a'b'^\dagger+a'^\dagger b'}}\\
  &{a'^\dagger}^{n-1} {b'^\dagger}^{n-1}
  \paren{a'^\dagger+b'^\dagger}|0, 0\rangle\\
  =&\frac{\cos\phi}{2n!\paren{n-1}!}
  \langle0, 0|
  {a'}^{n-1} {b'}^{n-1}
  \paren{a'+b'}
  \paren{a'^\dagger a'-b'^\dagger b'}{a'^\dagger}^{n-1} {b'^\dagger}^{n-1}
  \paren{a'^\dagger+b'^\dagger}|0, 0\rangle\\
  &-\frac{\sin\phi}{2n!\paren{n-1}!}
  \langle0, 0|
  {a'}^{n-1} {b'}^{n-1}
  \paren{a'+b'}
  \paren{a'b'^\dagger+a'^\dagger b'}{a'^\dagger}^{n-1} {b'^\dagger}^{n-1}
  \paren{a'^\dagger+b'^\dagger}|0, 0\rangle\\
  =&-n\sin\phi
  \intertext{Square}
  M^2=&\paren{\cos\phi\paren{a'^\dagger a'-b'^\dagger b'}-\sin\phi\paren{a'b'^\dagger+a'^\dagger b'}}^2\\
  =&\cos^2\phi\paren{a'^\dagger a'a'^\dagger a'-2a'^\dagger a'b'^\dagger b'+b'^\dagger b'b'^\dagger b'}+\sin^2\phi
  \paren{
    a'^2{b'^\dagger}^2+a'a'^\dagger b'^\dagger b'+a'^\dagger a'b'b'^\dagger+{a'^\dagger}^2b'^2
  }\\
  &
  -\sin\phi\cos\phi\paren{2a'^\dagger a'^2b'^\dagger+a'b'^\dagger
    +2{a'^\dagger}^2 a'b'+a'^\dagger b'
    -2a'{b'^\dagger}^2b'-a'b'^\dagger
    -2a'^\dagger{b'^\dagger}b'^2-a'^\dagger b'}\\
  =&\cos^2\phi\paren{a'^\dagger a'a'^\dagger a'-2a'^\dagger a'b'^\dagger b'+b'^\dagger b'b'^\dagger b'}+\sin^2\phi
  \paren{
    a'^2{b'^\dagger}^2+a'a'^\dagger b'^\dagger b'+a'^\dagger a'b'b'^\dagger+{a'^\dagger}^2b'^2
  }\\
  &-2\sin\phi\cos\phi\paren{a'^\dagger a'^2b'^\dagger+{a'^\dagger}^2 a'b'
    -a'{b'^\dagger}^2b'-a'^\dagger{b'^\dagger}b'^2}\\
  \angl{M^2}=&\cos^2\phi\angl{a'^\dagger a'a'^\dagger a'-2a'^\dagger a'b'^\dagger b'+b'^\dagger b'b'^\dagger b'}\\
  &+\sin^2\phi\angl{
    a'^2{b'^\dagger}^2+a'a'^\dagger b'^\dagger b'+a'^\dagger a'b'b'^\dagger+{a'^\dagger}^2b'^2
  }\\
  &-2\sin\phi\cos\phi\angl{a'^\dagger a'^2b'^\dagger+{a'^\dagger}^2 a'b'
    -a'{b'^\dagger}^2b'-a'^\dagger{b'^\dagger}b'^2}\\
  =&\frac{\cos^2\phi}{2n}\paren{n^3+\paren{n-1}^2n-2n^2\paren{n-1}-2n^2\paren{n-1}+\paren{n-1}^2n+n^3}\\
  &+\frac{\sin^2\phi}{2n}\paren{2\paren{n-1}n\paren{n+1}+2n^3}\\
  &-\frac{\sin\phi\cos\phi}{n}\paren{n^2\paren{n-1}+n^2\paren{n-1}
    -n^2\paren{n-1}-n^2\paren{n-1}}\\
  =&\cos^2\phi+\sin^2\phi\paren{2n^2-1}
  \intertext{Fluctuation}
  \Delta M^2=&\cos^2\phi+\sin^2\phi\paren{2n^2-1}-n^2\sin^2\phi\\
  =&\cos^2\phi+\sin^2\phi\paren{n^2-1}\\
  \pdiff{\angl{M}}{\phi}=&-n\cos\phi\\
  \Delta \phi^2=&\frac{\cos^2\phi+\sin^2\phi\paren{n^2-1}}{n^2\cos^2\phi}\\
  =&\frac{1+\tan^2\phi\paren{n^2-1}}{n^2}\\
  \Delta \phi=&\frac{\sqrt{1+\tan^2\phi\paren{n^2-1}}}{n}
  \intertext{for $\phi=0$}
  \Delta \phi=&\frac{1}{n}
}
\subsection{}
\eqar{
  |\psi_0\rangle=&\left|\alpha, 0\right\rangle\\
  |\psi_1\rangle=&\left|\frac{\alpha}{\sqrt{2}}, -\frac{\ui\alpha}{\sqrt{2}}\right\rangle\\
  |\psi_2\rangle=&\left|\frac{\alpha\ue^{-\ui\phi}}{\sqrt{2}}, -\frac{\ui\alpha}{\sqrt{2}}\right\rangle\\
  |\psi_3\rangle=&\left|\frac{\alpha\ue^{-\ui\phi}}{2}+\frac{\alpha}{2}, \ui\paren{\frac{\alpha\ue^{-\ui\phi}}{2}-\frac{\alpha}{2}}\right\rangle\\
  =&\left|\alpha\ue^{-{\ui\phi}/{2}}\cos\frac{\phi}{2},
    \alpha\ue^{-{\ui\phi}/{2}}\sin\frac{\phi}{2}\right\rangle
}
\subsection{}
Mean
\eqar{
  \angl{M}=&\angl{a^\dagger a-b^\dagger b}\\
  =&\alpha^*\ue^{{\ui\phi}/{2}}\cos\frac{\phi}{2}\alpha\ue^{-{\ui\phi}/{2}}\cos\frac{\phi}{2}-\alpha^*\ue^{{\ui\phi}/{2}}\sin\frac{\phi}{2} \alpha\ue^{-{\ui\phi}/{2}}\sin\frac{\phi}{2}\\
  =&\abs{\alpha}^2\cos^2\frac{\phi}{2}-\alpha^2\sin^2\frac{\phi}{2}\\
  =&\abs{\alpha}^2\cos\phi
  \intertext{Square}
  \angl{M^2}=&\angl{\paren{a^\dagger a-b^\dagger b}
    \paren{a^\dagger a-b^\dagger b}}\\
  =&\angl{a^\dagger aa^\dagger a-a^\dagger ab^\dagger b-b^\dagger ba^\dagger a+b^\dagger bb^\dagger b}\\
  =&\angl{M}^2+\angl{a^\dagger a+b^\dagger b}\\
  =&\angl{M}^2+\abs{\alpha}^2
  \intertext{Uncertainty}
  \angl{\Delta\phi^2}=&\frac{\abs{\alpha}^2}{\abs{\alpha}^4\sin^2\phi}\\
  =&\frac{1}{\abs{\alpha}^2\sin^2\phi}
}

\section{}
\subsection{}
\eqar{
  P=&\abs{\psi_A}^2\abs{\psi_B}^2\abs{\ue^{\ui\paren{\vec k_A\cdot\vec r_{A1}+\vec k_B\cdot\vec r_{B2}}}\pm\ue^{\ui\paren{\vec k_A\cdot\vec r_{A2}+\vec k_B\cdot\vec r_{B1}}}}^2\\
  =&\abs{\psi_A}^2\abs{\psi_B}^2\abs{\ue^{\ui\vec k_A\cdot\vec r_{21}}\pm\ue^{\ui\vec k_B\cdot\vec r_{21}}}^2\\
  =&\abs{\psi_A}^2\abs{\psi_B}^2\abs{\ue^{\ui\paren{\vec k_A-\vec k_B}\cdot\vec r_{21}/2}\pm\ue^{-\ui\paren{\vec k_A-\vec k_B}\cdot\vec r_{21}/2}}^2\\
  =&\abs{\psi_A}^2\abs{\psi_B}^2\abs{2\pm\ue^{\ui\paren{\vec k_A-\vec k_B}\cdot\vec r_{21}}\pm\ue^{-\ui\paren{\vec k_A-\vec k_B}\cdot\vec r_{21}}}\\
  =&2\abs{\psi_A}^2\abs{\psi_B}^2\paren{1\pm\cos\paren{\paren{\vec k_A-\vec k_B}\cdot\vec r_{21}}}
}
\subsection{}
In order to see the correlation $\Delta\phi_t\ll1$,
\eqar{
  1\gg&\Delta \vec k_t\cdot\vec r_{21t}\\
  =&k_0\frac{W}{d}w\\
  =&\frac{2\pi Ww}{\lambda d}\\
  \lambda d\gg&Ww
}
For $^{6}\text{Li}$ at $500\mu\text{K}$
\eqar{
  \lambda=&\frac{\hbar}{p}\\
  =&\frac{\hbar}{\sqrt{mk_BT}}\\
  \approx&12\text{nm}\\
  w_{max}\approx&\sqrt{\lambda d}\\
  \approx&36\mu\text{m}
}
\subsection{}
\subsubsection{}
\eqar{
  \angl{P}=&2\abs{\psi_A}^2\abs{\psi_B}^2\sqrt{\frac{\gamma}{\pi}}\int\paren{1\pm\cos\Delta k_r r_{21}}\ue^{-\Delta k_r^2\gamma^2}\ud\Delta k_r\\
  =&2\abs{\psi_A}^2\abs{\psi_B}^2\paren{1\pm\exp\paren{-\frac{r^2_{21}}{4\gamma^2}}}\\
  =&2\abs{\psi_A}^2\abs{\psi_B}^2\paren{1\pm\exp\paren{-\frac{r^2_{21l}+r^2_{21t}}{4\gamma^2}}}
}
\begin{tikzpicture}
  \draw[blue] (0, 0) plot[domain=-3:3, samples=1000] function {1 + exp(-x*x / 2)};
  \draw[red] (0, 0) plot[domain=-3:3, samples=1000] function {1 - exp(-x*x / 2)};
  \draw[->, line width=1] (-3.5, 0) -- (3.5, 0) node[below] {$r_{21}$};
  \draw[->, line width=1] (0, 0) -- (0, 2.5) node[right] {$\angl{P}$};
  \path (3, 1) node[blue, above] {Boson};
  \path (3, 1) node[red, below] {Fermion};
\end{tikzpicture}

\subsubsection{}
\eqar{
  \Delta k=&\frac{\Delta p}{\hbar}\\
  =&\frac{m}{\hbar}\Delta v\\
  =&\frac{m}{\hbar}\Delta\paren{\frac{d}{\tau}}\\
  =&\frac{mL}{\hbar\tau}\\
  =&\frac{mLv}{\hbar d}
}
\eqar{
  % \gamma=&\frac{\hbar}{\sqrt{mk_BT}}\\
  % =&12.7\text{nm}\\
  vt_{min}<&\frac{\hbar d}{mvL}\\
  t_{min}<&\frac{\hbar\tau^2}{mdL}\\
  =&\frac{\hbar\tau^2}{mdL}\\
  \approx&35\mu\text{s}
}

\subsection{}

\end{document}
